doc/coq/Concrete.v
@@ -1,45 +1,4 @@
-From Coq Require Export Bool.Bool.
-From Coq Require Export Init.Nat.
-From Coq Require Export Arith.Arith.
-From Coq Require Export Arith.EqNat.
-From Coq Require Export Lia.
-From Coq Require Export Lists.List.
-From Coq Require Export Strings.String.
-
-Notation "x :: y" := (cons x y)
-                     (at level 60, right associativity).
-Notation "[ ]" := nil.
-Notation "[ x ; .. ; y ]" := (cons x .. (cons y []) ..).
-Notation "x ++ y" := (app x y)
-                     (at level 60, right associativity).
-
-Inductive expr_id :=
-  | eid (x : nat)
-.
-
-Inductive mod_id :=
-  | mid (M : nat)
-.
-
-Inductive mod_tm :=
-  | m_empty
-  | m_var (M : mod_id)
-  | m_lete (x : expr_id) (e : expr_tm) (m : mod_tm)
-  | m_letm (M : mod_id) (m1 : mod_tm) (m2 : mod_tm)
-
-with expr_tm :=
-  | e_var (x : expr_id)
-  | e_lam (x : expr_id) (e : expr_tm)
-  | e_app (e1 : expr_tm) (e2 : expr_tm)
-  | e_link (m : mod_tm) (e : expr_tm)
-.
-
-Inductive value : expr_tm -> Prop :=
-  | v_fn (x : expr_id) (e : expr_tm) : value (e_lam x e)
-.
-
-Scheme expr_ind_mut := Induction for expr_tm Sort Prop
-with mod_ind_mut := Induction for mod_tm Sort Prop.
+Require Export Modular.Syntax.
 
 Definition time := nat.
 
@@ -1371,4 +1330,3 @@ Proof.
     destruct FINAL as [MEM KILLER].
     apply KILLER. apply collect_ctx_expr_refl.
 Qed.
-(* Soundness of big-step relation : equivalence to definitional interpreter with fuel *)
