doc/coq/Abstract.v
@@ -1,0 +1,1364 @@
+Require Export Modular.Syntax.
+
+Definition time := nat.
+
+Definition path := list time.
+
+Definition update_t (t : time) := S t.
+
+Definition eq_t (t1 t2 : time) := t1 =? t2.
+
+Fixpoint eq_p (p1 p2 : path) :=
+  match p1, p2 with
+  | [], [] => true
+  | hd1 :: tl1, [] => false
+  | [], hd2 :: tl2 => false
+  | hd1 :: tl1, hd2 :: tl2 =>
+    if eq_t hd1 hd2 then eq_p tl1 tl2
+                    else false
+  end.
+
+Definition len_p (p : path) := List.length p.
+
+Inductive dy_ctx :=
+  | dy_c_hole
+  | dy_c_lam (x: expr_id) (tx : time) (C : dy_ctx)
+  | dy_c_lete (x : expr_id) (tx : time) (C : dy_ctx)
+  | dy_c_letm (M : mod_id) (CM : dy_ctx) (C : dy_ctx)
+.
+
+Fixpoint dy_plugin_c Cout Cin :=
+  match Cout with
+  | dy_c_hole => Cin
+  | dy_c_lam x tx C' => dy_c_lam x tx (dy_plugin_c C' Cin)
+  | dy_c_lete x tx C' => dy_c_lete x tx (dy_plugin_c C' Cin)
+  | dy_c_letm M CM C' => dy_c_letm M CM (dy_plugin_c C' Cin)
+  end.
+
+Definition eq_eid id1 id2 :=
+  match id1, id2 with
+  | eid x1, eid x2 => x1 =? x2
+  end.
+
+Definition eq_mid id1 id2 :=
+  match id1, id2 with
+  | mid M1, mid M2 => M1 =? M2
+  end.
+
+Fixpoint dy_level (C : dy_ctx) : path :=
+  match C with
+  | dy_c_hole => []
+  | dy_c_lam _ t C'
+  | dy_c_lete _ t  C' => t :: dy_level C'
+  | dy_c_letm _ _  C' => dy_level C'
+  end.
+
+Fixpoint addr_x (C : dy_ctx) (x : expr_id) :=
+  match C with
+  | dy_c_hole => []
+  | dy_c_lam x' tx' C'
+  | dy_c_lete x' tx' C' =>
+    match addr_x C' x with
+    | [] => if eq_eid x x' then [tx'] else []
+    | addr => tx' :: addr
+    end
+  | dy_c_letm _ _ C' => addr_x C' x
+  end.
+
+Fixpoint ctx_M (C : dy_ctx) (M : mod_id) :=
+  match C with
+  | dy_c_hole => None
+  | dy_c_lam _ _ C'
+  | dy_c_lete _ _ C' => ctx_M C' M
+  | dy_c_letm M' CM' C' =>
+    match ctx_M C' M with
+    | Some CM => Some CM
+    | None => if eq_mid M M' then Some CM' else None
+    end
+  end.
+
+(* a term, a proof, a path, a context *)
+Inductive expr_value :=
+  | Val (v : expr_tm) (pf : value v) (C : dy_ctx)
+.
+
+Inductive state :=
+  | ST (mem : path -> option (list expr_value))
+       (t : time)
+.
+
+Definition update_m {X} mem (p : path) (x : X) :=
+  fun p1 => 
+  if eq_p p1 p then
+    match mem p with
+      | Some l => Some (x :: l)
+      | None => Some [x]
+    end
+  else mem p1.
+
+Definition empty_mem {X} (p : path) : option X := None.
+
+Notation "p '!->' v ';' mem" := (update_m mem p v)
+                              (at level 100, v at next level, right associativity).
+
+Notation "Cout '[|' Cin '|]'" := (dy_plugin_c Cout Cin)
+                              (at level 100, Cin at next level, right associativity).
+Notation "'[||]'" := (dy_c_hole) (at level 100).
+
+Inductive EevalR (C : dy_ctx) (st : state)
+    : expr_tm -> expr_value -> state -> Prop :=
+  | Eeval_var x vl v mem t
+             (STATE : ST mem t = st)
+             (ADDR : [] <> addr_x C x)
+             (ACCESS : Some vl = mem (addr_x C x))
+             (IN : In v vl)
+    : EevalR C st (e_var x) v st
+  | Eeval_lam x e
+    : EevalR C st (e_lam x e)
+            (Val (e_lam x e) (v_fn x e) C) st
+  | Eeval_app e1 e2 
+              x e C_lam st_lam
+              arg mem t
+              v st_v
+              (FN : EevalR C st e1
+                           (Val (e_lam x e) (v_fn x e) C_lam) st_lam)
+              (ARG : EevalR C st_lam e2
+                            arg (ST mem t))
+              (BODY : EevalR (C_lam [|dy_c_lam x t  ([||])|])
+                             (ST ((dy_level C_lam) ++ [t] !-> arg ; mem) (update_t t))
+                              e v st_v)
+    : EevalR C st (e_app e1 e2) v st_v
+  | Eeval_link m e C_m st_m v st_v
+               (MOD : MevalR C st m C_m st_m)
+               (LINK : EevalR C_m st_m e v st_v)
+    : EevalR C st (e_link m e) v st_v
+
+with MevalR (C : dy_ctx) (st : state)
+    : mod_tm -> dy_ctx -> state -> Prop :=
+  | Meval_empty
+    : MevalR C st m_empty C st
+  | Meval_var M C_M (ACCESS : Some C_M = ctx_M C M)
+    : MevalR C st (m_var M) C_M st
+  | Meval_lete x e v_e mem t
+               m C_m st_m
+               (EVALe : EevalR C st e v_e (ST mem t))
+               (EVALm : MevalR (C [|dy_c_lete x t  ([||])|]) 
+                        (ST ((dy_level C ++ [t]) !-> v_e ; mem) (update_t t))
+                        m C_m st_m)
+    : MevalR C st (m_lete x e m) C_m st_m
+  | Meval_letm M m1 C_m1 st_m1
+               m2 C_m2 st_m2
+               (EVALm1 : MevalR C st m1 C_m1 st_m1)
+               (EVALm2 : MevalR (C [|dy_c_letm M C_m1  ([||])|]) st_m1
+                         m2 C_m2 st_m2)
+    : MevalR C st (m_letm M m1 m2) C_m2 st_m2
+.
+
+Scheme EevalR_ind_mut := Induction for EevalR Sort Prop
+with MevalR_ind_mut := Induction for MevalR Sort Prop.
+
+Definition Reach (tm1 tm2 : Type) := tm1 -> dy_ctx -> state -> tm2 -> Prop.
+
+(* Reachability relation, sensible version *)
+Inductive _EreachE (C : dy_ctx) (st : state)
+    : Reach expr_tm expr_tm :=
+  | _ere_refl e
+    : _EreachE C st e 
+               C st e
+  | _ere_var x mem t vl v pf C_v
+            (STATE : ST mem t = st)
+            (ADDR : [] <> addr_x C x)
+            (ACCESS : Some vl = mem (addr_x C x))
+            (IN : In (Val v pf C_v) vl)
+    : _EreachE C st (e_var x) 
+               C_v st v
+  | _ere_app_left e1 e2 C' st' e'
+                 (REACHl : _EreachE C st e1
+                                    C' st' e')
+    : _EreachE C st (e_app e1 e2) 
+               C' st' e'
+  | _ere_app_right e1 e2 st1 v C' st' e'
+                  (FN : EevalR C st e1 v st1)
+                  (REACHr : _EreachE C st1 e2
+                                     C' st' e')
+    : _EreachE C st (e_app e1 e2)
+               C' st' e'
+  | _ere_app_body e1 e2 x e C_lam st_lam
+                 arg mem t
+                 C' st' e'
+                 (FN : EevalR C st e1 
+                             (Val (e_lam x e) (v_fn x e) C_lam) st_lam)
+                 (ARG : EevalR C st_lam e2
+                               arg (ST mem t))
+                 (REACHb : _EreachE (C_lam[|dy_c_lam x t  ([||])|]) 
+                                    (ST ((dy_level C_lam ++ [t]) !-> arg ; mem) (update_t t)) e
+                                     C' st' e')
+    : _EreachE C st (e_app e1 e2)
+               C' st' e'
+  | _ere_link_m m e C' st' e'
+               (REACHm : _MreachE C st m
+                                  C' st' e')
+    : _EreachE C st (e_link m e)
+               C' st' e'
+  | _ere_link_e m e C_m st_m C' st' e'
+               (MOD : MevalR C st m C_m st_m)
+               (REACHe : _EreachE C_m st_m e
+                                  C' st' e')
+    : _EreachE C st (e_link m e)
+               C' st' e'
+
+with _MreachE (C : dy_ctx) (st : state)
+    : Reach mod_tm expr_tm :=
+  | _mre_lete_e x e m C' st' e'
+               (REACHe : _EreachE C st e
+                                  C' st' e')
+    : _MreachE C st (m_lete x e m)
+               C' st' e'
+  | _mre_lete_m x e m v mem t
+                C' st' e'
+             (EVALx : EevalR C st e v (ST mem t))
+             (REACHm : _MreachE (C[|dy_c_lete x t  ([||])|])
+                                (ST ((dy_level C ++ [t]) !-> v ; mem) (update_t t)) m
+                                 C' st' e')
+    : _MreachE C st (m_lete x e m)
+               C' st' e'
+  | _mre_letm_m1 M m1 m2 C' st' e'
+               (REACHm : _MreachE C st m1
+                                  C' st' e')
+    : _MreachE C st (m_letm M m1 m2)
+               C' st' e'
+  | _mre_letm_m2 M m1 m2 C_M st_M
+                 C' st' e'
+             (EVALM : MevalR C st m1 C_M st_M)
+             (REACHm : _MreachE (C[|dy_c_letm M C_M  ([||])|]) st_M m2
+                                 C' st' e')
+    : _MreachE C st (m_letm M m1 m2)
+               C' st' e'.
+
+Scheme __EreachE_ind_mut := Induction for _EreachE Sort Prop
+with __MreachE_ind_mut := Induction for _MreachE Sort Prop.
+
+Inductive _MreachM (C : dy_ctx) (st : state)
+    : Reach mod_tm mod_tm :=
+  | _mrm_refl m
+    : _MreachM C st m
+               C st m
+  | _mrm_var M C_M (ACCESS : Some C_M = ctx_M C M)
+    : _MreachM C st (m_var M)
+               C_M st m_empty
+  | _mrm_lete_e x e m C' st' m'
+               (REACHe : _EreachM C st e
+                                  C' st' m')
+    : _MreachM C st (m_lete x e m)
+               C' st' m'
+  | _mrm_lete_m x e m v mem t
+                C' st' m'
+             (EVALx : EevalR C st e v (ST mem t))
+             (REACHm : _MreachM (C[|dy_c_lete x t  ([||])|]) 
+                                (ST ((dy_level C ++ [t]) !-> v ; mem) (update_t t)) m
+                                 C' st' m')
+    : _MreachM C st (m_lete x e m)
+               C' st' m'
+  | _mrm_letm_m1 M m1 m2 C' st' m'
+               (REACHm : _MreachM C st m1
+                                  C' st' m')
+    : _MreachM C st (m_letm M m1 m2)
+               C' st' m'
+  | _mrm_letm_m2 M m1 m2 C_M st_M
+                 C' st' m'
+             (EVALM : MevalR C st m1 C_M st_M)
+             (REACHm : _MreachM (C[|dy_c_letm M C_M  ([||])|]) st_M m2
+                                 C' st' m')
+    : _MreachM C st (m_letm M m1 m2)
+               C' st' m'
+
+with _EreachM (C : dy_ctx) (st : state)
+    : Reach expr_tm mod_tm :=
+  | _erm_app_left e1 e2 C' st' m'
+                 (REACHl : _EreachM C st e1
+                                    C' st' m')
+    : _EreachM C st (e_app e1 e2) 
+               C' st' m'
+  | _erm_app_right e1 e2 v1 st1 C' st' m'
+                  (FN : EevalR C st e1 v1 st1)
+                  (REACHr : _EreachM C st1 e2
+                                     C' st' m')
+    : _EreachM C st (e_app e1 e2)
+               C' st' m'
+  | _erm_app_body e1 e2 x e C_lam st_lam
+                 arg mem t
+                 C' st' m'
+                 (FN : EevalR C st e1 
+                              (Val (e_lam x e) (v_fn x e) C_lam) st_lam)
+                 (ARG : EevalR C st_lam e2 arg (ST mem t))
+                 (REACHb : _EreachM (C_lam[|dy_c_lam x t ([||])|]) 
+                                    (ST ((dy_level C_lam ++ [t]) !-> arg ; mem) (update_t t)) e
+                                     C' st' m')
+    : _EreachM C st (e_app e1 e2)
+               C' st' m'
+  | _erm_link_m m e C' st' m'
+               (REACHm : _MreachM C st m
+                                  C' st' m')
+    : _EreachM C st (e_link m e)
+               C' st' m'
+  | _erm_link_e m e C_m st_m C' st' m'
+               (MOD : MevalR C st m C_m st_m)
+               (REACHe : _EreachM C_m st_m e
+                                  C' st' m')
+    : _EreachM C st (e_link m e)
+               C' st' m'
+.
+
+Scheme __EreachM_ind_mut := Induction for _EreachM Sort Prop
+with __MreachM_ind_mut := Induction for _MreachM Sort Prop.
+
+(* for proofs *)
+Inductive EreachE (C : dy_ctx) (st : state)
+    : Reach expr_tm expr_tm :=
+  | ere_refl e
+    : EreachE C st e 
+              C st e
+  | ere_var x mem t vl v pf C_v
+            (STATE : ST mem t = st)
+            (ADDR : [] <> addr_x C x)
+            (ACCESS : Some vl = mem (addr_x C x))
+            (IN : In (Val v pf C_v) vl)
+    : EreachE C st (e_var x) 
+              C_v st v
+  | ere_app_left e1 e2 C' st' e'
+                 (REACHl : EreachE C st e1
+                                   C' st' e')
+    : EreachE C st (e_app e1 e2) 
+              C' st' e'
+  | ere_app_right e1 e2 st_lam v pf C_lam C' st' e'
+                  (FN : EevalR C st e1 (Val v pf C_lam) st_lam)
+                  (FNr : EreachE C st e1 C_lam st_lam v)
+                  (REACHr : EreachE C st_lam e2
+                                    C' st' e')
+    : EreachE C st (e_app e1 e2)
+              C' st' e'
+  | ere_app_body e1 e2 x e C_lam st_lam
+                 arg pf C_arg mem t
+                 C' st' e'
+                 (FN : EevalR C st e1 
+                             (Val (e_lam x e) (v_fn x e) C_lam) st_lam)
+                 (FNr : EreachE C st e1 C_lam st_lam (e_lam x e))
+                 (ARG : EevalR C st_lam e2
+                               (Val arg pf C_arg) (ST mem t))
+                 (ARGr : EreachE C st_lam e2 C_arg (ST mem t) arg)
+                 (REACHb : EreachE (C_lam[|dy_c_lam x t ([||])|]) 
+                                    (ST ((dy_level C_lam ++ [t]) !-> (Val arg pf C_arg) ; mem) (update_t t)) e
+                                     C' st' e')
+    : EreachE C st (e_app e1 e2)
+              C' st' e'
+  | ere_link_m m e C' st' e'
+               (REACHm : MreachE C st m
+                                 C' st' e')
+    : EreachE C st (e_link m e)
+              C' st' e'
+  | ere_link_e m e C_m st_m C' st' e'
+              (MOD : MevalR C st m C_m st_m)
+              (MODr : MreachM C st m C_m st_m m_empty)
+              (REACHe : EreachE C_m st_m e
+                                C' st' e')
+    : EreachE C st (e_link m e)
+              C' st' e'
+
+with MreachE (C : dy_ctx) (st : state)
+    : Reach mod_tm expr_tm :=
+  | mre_lete_e x e m C' st' e'
+               (REACHe : EreachE C st e
+                                 C' st' e')
+    : MreachE C st (m_lete x e m)
+              C' st' e'
+  | mre_lete_m x e m v pf C_x mem t
+               C' st' e'
+             (EVALx : EevalR C st e (Val v pf C_x) (ST mem t))
+             (EVALxr : EreachE C st e C_x (ST mem t) v)
+             (REACHm : MreachE (C[|dy_c_lete x t ([||])|])
+                                (ST ((dy_level C ++ [t]) !-> (Val v pf C_x) ; mem) (update_t t)) m
+                                 C' st' e')
+    : MreachE C st (m_lete x e m)
+              C' st' e'
+  | mre_letm_m1 M m1 m2 C' st' e'
+              (REACHm : MreachE C st m1
+                                C' st' e')
+    : MreachE C st (m_letm M m1 m2)
+              C' st' e'
+  | mre_letm_m2 M m1 m2 C_M st_M
+                C' st' e'
+             (EVALM : MevalR C st m1 C_M st_M)
+             (EVALM : MreachM C st m1 C_M st_M m_empty)
+             (REACHm : MreachE (C[|dy_c_letm M C_M ([||])|]) st_M m2
+                                C' st' e')
+    : MreachE C st (m_letm M m1 m2)
+              C' st' e'
+
+with MreachM (C : dy_ctx) (st : state)
+    : Reach mod_tm mod_tm :=
+  | mrm_refl m
+    : MreachM C st m
+              C st m
+  | mrm_var M C_M (ACCESS : Some C_M = ctx_M C M)
+    : MreachM C st (m_var M)
+              C_M st m_empty
+  | mrm_lete_e x e m C' st' m'
+               (REACHe : EreachM C st e
+                                  C' st' m')
+    : MreachM C st (m_lete x e m)
+              C' st' m'
+  | mrm_lete_m x e m v pf C_x mem t
+               C' st' m'
+             (EVALx : EevalR C st e (Val v pf C_x) (ST mem t))
+             (EVALxr : EreachE C st e C_x (ST mem t) v)
+             (REACHm : MreachM (C[|dy_c_lete x t ([||])|]) 
+                               (ST ((dy_level C ++ [t]) !-> (Val v pf C_x) ; mem) (update_t t)) m
+                                C' st' m')
+    : MreachM C st (m_lete x e m)
+              C' st' m'
+  | mrm_letm_m1 M m1 m2 C' st' m'
+               (REACHm : MreachM C st m1
+                                 C' st' m')
+    : MreachM C st (m_letm M m1 m2)
+              C' st' m'
+  | mrm_letm_m2 M m1 m2 C_M st_M
+                C' st' m'
+             (EVALM : MevalR C st m1 C_M st_M)
+             (EVALMr : MreachM C st m1 C_M st_M m_empty)
+             (REACHm : MreachM (C[|dy_c_letm M C_M  ([||])|]) st_M m2
+                                C' st' m')
+    : MreachM C st (m_letm M m1 m2)
+              C' st' m'
+
+with EreachM (C : dy_ctx) (st : state)
+    : Reach expr_tm mod_tm :=
+  | erm_app_left e1 e2 C' st' m'
+                (REACHl : EreachM C st e1
+                                  C' st' m')
+    : EreachM C st (e_app e1 e2) 
+              C' st' m'
+  | erm_app_right e1 e2 v pf C_lam st_lam C' st' m'
+                 (FN : EevalR C st e1 (Val v pf C_lam) st_lam)
+                 (FNr : EreachE C st e1 C_lam st_lam v)
+                 (REACHr : EreachM C st_lam e2
+                                   C' st' m')
+    : EreachM C st (e_app e1 e2)
+              C' st' m'
+  | erm_app_body e1 e2 x e C_lam st_lam
+                 arg pf C_arg mem t
+                 C' st' m'
+                 (FN : EevalR C st e1 
+                              (Val (e_lam x e) (v_fn x e) C_lam) st_lam)
+                 (FNr : EreachE C st e1 
+                                C_lam st_lam (e_lam x e))
+                 (ARG : EevalR C st_lam e2 (Val arg pf C_arg) (ST mem t))
+                 (ARGr : EreachE C st_lam e2 C_arg (ST mem t) arg)
+                 (REACHb : EreachM (C_lam[|dy_c_lam x t ([||])|]) 
+                                   (ST ((dy_level C_lam ++ [t]) !-> (Val arg pf C_arg) ; mem) (update_t t)) e
+                                    C' st' m')
+    : EreachM C st (e_app e1 e2)
+              C' st' m'
+  | erm_link_m m e C' st' m'
+              (REACHm : MreachM C st m
+                                C' st' m')
+    : EreachM C st (e_link m e)
+              C' st' m'
+  | erm_link_e m e C_m st_m C' st' m'
+              (MOD : MevalR C st m C_m st_m)
+              (MODr : MreachM C st m C_m st_m m_empty)
+              (REACHe : EreachM C_m st_m e
+                                C' st' m')
+    : EreachM C st (e_link m e)
+              C' st' m'
+.
+
+Scheme _EreachE_ind_mut := Induction for EreachE Sort Prop
+with _EreachM_ind_mut := Induction for EreachM Sort Prop
+with _MreachE_ind_mut := Induction for MreachE Sort Prop
+with _MreachM_ind_mut := Induction for MreachM Sort Prop.
+
+Notation "'<e|' C1 st1 tm1 '~>' C2 st2 tm2 '|e>'" := (EreachE C1 st1 tm1 C2 st2 tm2) 
+                                               (at level 10, 
+                                                C1 at next level, st1 at next level, tm1 at next level,
+                                                C2 at next level, st2 at next level, tm2 at next level).
+
+Notation "'<m|' C1 st1 tm1 '~>' C2 st2 tm2 '|e>'" := (MreachE C1 st1 tm1 C2 st2 tm2) 
+                                               (at level 10, 
+                                                C1 at next level, st1 at next level, tm1 at next level,
+                                                C2 at next level, st2 at next level, tm2 at next level).
+
+Notation "'<m|' C1 st1 tm1 '~>' C2 st2 tm2 '|m>'" := (MreachM C1 st1 tm1 C2 st2 tm2) 
+                                               (at level 10, 
+                                                C1 at next level, st1 at next level, tm1 at next level,
+                                                C2 at next level, st2 at next level, tm2 at next level).
+
+Notation "'<e|' C1 st1 tm1 '~>' C2 st2 tm2 '|m>'" := (EreachM C1 st1 tm1 C2 st2 tm2) 
+                                               (at level 10, 
+                                                C1 at next level, st1 at next level, tm1 at next level,
+                                                C2 at next level, st2 at next level, tm2 at next level).
+
+(* sanity check *)
+Lemma ere_trans : forall C1 st1 e1
+                         C2 st2 e2
+                         C3 st3 e3
+                         (REACH1 : <e| C1 st1 e1 ~> C2 st2 e2 |e>)
+                         (REACH2 : <e| C2 st2 e2 ~> C3 st3 e3 |e>),
+                         <e| C1 st1 e1 ~> C3 st3 e3 |e>.
+Proof.
+  intros. generalize dependent e3.
+  revert C3 st3.
+  apply (_EreachE_ind_mut
+    (fun C1 st1 e1 
+         C2 st2 e2 
+         (REACH1 : <e| C1 st1 e1 ~> C2 st2 e2 |e>)=> 
+         forall C3 st3 e3 
+                (REACH2 : <e| C2 st2 e2 ~> C3 st3 e3 |e>),
+                <e| C1 st1 e1 ~> C3 st3 e3 |e>)
+    (fun C1 st1 e1 
+         C2 st2 m2 
+         (REACH1 : <e| C1 st1 e1 ~> C2 st2 m2 |m>)=> 
+         forall C3 st3 e3 
+                (REACH2 : <m| C2 st2 m2 ~> C3 st3 e3 |e>),
+                <e| C1 st1 e1 ~> C3 st3 e3 |e>)
+    (fun C1 st1 m1
+         C2 st2 e2
+         (REACH1 : <m| C1 st1 m1 ~> C2 st2 e2 |e>) =>
+         forall C3 st3 e3 
+                (REACH2 : <e| C2 st2 e2 ~> C3 st3 e3 |e>),
+                <m| C1 st1 m1 ~> C3 st3 e3 |e>)
+    (fun C1 st1 m1 
+         C2 st2 m2 
+         (REACH1 : <m| C1 st1 m1 ~> C2 st2 m2 |m>)=> 
+         forall C3 st3 e3 
+                (REACH2 : <m| C2 st2 m2 ~> C3 st3 e3 |e>),
+                <m| C1 st1 m1 ~> C3 st3 e3 |e>));
+   eauto using EreachE, EreachM, MreachE, MreachM;
+   intros; try inversion pf; subst; inversion REACH2; subst;
+   eauto using EreachE, EreachM, MreachE, MreachM.
+Qed.
+
+Lemma mrm_trans : forall C1 st1 m1
+                         C2 st2 m2
+                         C3 st3 m3
+                         (REACH1 : <m| C1 st1 m1 ~> C2 st2 m2 |m>)
+                         (REACH2 : <m| C2 st2 m2 ~> C3 st3 m3 |m>),
+                         <m| C1 st1 m1 ~> C3 st3 m3 |m>.
+Proof.
+  intros. generalize dependent m3.
+  revert C3 st3.
+  apply (_MreachM_ind_mut
+    (fun C1 st1 e1 
+         C2 st2 e2 
+         (REACH1 : <e| C1 st1 e1 ~> C2 st2 e2 |e>)=> 
+         forall C3 st3 m3 
+                (REACH2 : <e| C2 st2 e2 ~> C3 st3 m3 |m>),
+                <e| C1 st1 e1 ~> C3 st3 m3 |m>)
+    (fun C1 st1 e1 
+         C2 st2 m2 
+         (REACH1 : <e| C1 st1 e1 ~> C2 st2 m2 |m>)=> 
+         forall C3 st3 m3 
+                (REACH2 : <m| C2 st2 m2 ~> C3 st3 m3 |m>),
+                <e| C1 st1 e1 ~> C3 st3 m3 |m>)
+    (fun C1 st1 m1
+         C2 st2 e2
+         (REACH1 : <m| C1 st1 m1 ~> C2 st2 e2 |e>) =>
+         forall C3 st3 m3 
+                (REACH2 : <e| C2 st2 e2 ~> C3 st3 m3 |m>),
+                <m| C1 st1 m1 ~> C3 st3 m3 |m>)
+    (fun C1 st1 m1 
+         C2 st2 m2 
+         (REACH1 : <m| C1 st1 m1 ~> C2 st2 m2 |m>)=> 
+         forall C3 st3 m3 
+                (REACH2 : <m| C2 st2 m2 ~> C3 st3 m3 |m>),
+                <m| C1 st1 m1 ~> C3 st3 m3 |m>));
+   eauto using EreachE, EreachM, MreachE, MreachM;
+   intros; try inversion pf; subst; inversion REACH2; subst;
+   eauto using EreachE, EreachM, MreachE, MreachM.
+Qed.
+
+Lemma ermre_trans : forall C1 st1 e1
+                           C2 st2 m2
+                           C3 st3 e3
+                           (REACH1 : <e| C1 st1 e1 ~> C2 st2 m2 |m>)
+                           (REACH2 : <m| C2 st2 m2 ~> C3 st3 e3 |e>),
+                           <e| C1 st1 e1 ~> C3 st3 e3 |e>. 
+Proof.
+  intros. generalize dependent e3.
+  revert C3 st3.
+  apply (_EreachM_ind_mut
+    (fun C1 st1 e1 
+         C2 st2 e2 
+         (REACH1 : <e| C1 st1 e1 ~> C2 st2 e2 |e>)=> 
+         forall C3 st3 e3 
+                (REACH2 : <e| C2 st2 e2 ~> C3 st3 e3 |e>),
+                <e| C1 st1 e1 ~> C3 st3 e3 |e>)
+    (fun C1 st1 e1 
+         C2 st2 m2 
+         (REACH1 : <e| C1 st1 e1 ~> C2 st2 m2 |m>)=> 
+         forall C3 st3 e3 
+                (REACH2 : <m| C2 st2 m2 ~> C3 st3 e3 |e>),
+                <e| C1 st1 e1 ~> C3 st3 e3 |e>)
+    (fun C1 st1 m1
+         C2 st2 e2
+         (REACH1 : <m| C1 st1 m1 ~> C2 st2 e2 |e>) =>
+         forall C3 st3 e3 
+                (REACH2 : <e| C2 st2 e2 ~> C3 st3 e3 |e>),
+                <m| C1 st1 m1 ~> C3 st3 e3 |e>)
+    (fun C1 st1 m1 
+         C2 st2 m2 
+         (REACH1 : <m| C1 st1 m1 ~> C2 st2 m2 |m>)=> 
+         forall C3 st3 e3 
+                (REACH2 : <m| C2 st2 m2 ~> C3 st3 e3 |e>),
+                <m| C1 st1 m1 ~> C3 st3 e3 |e>));
+   eauto using EreachE, EreachM, MreachE, MreachM;
+   intros; try inversion pf; subst; inversion REACH2; subst;
+   eauto using EreachE, EreachM, MreachE, MreachM.
+Qed.
+
+Lemma mrerm_trans : forall C1 st1 m1
+                           C2 st2 e2
+                           C3 st3 m3
+                           (REACH1 : <m| C1 st1 m1 ~> C2 st2 e2 |e>)
+                           (REACH2 : <e| C2 st2 e2 ~> C3 st3 m3 |m>),
+                           <m| C1 st1 m1 ~> C3 st3 m3 |m>. 
+Proof.
+  intros. generalize dependent m3.
+  revert C3 st3.
+  apply (_MreachE_ind_mut
+    (fun C1 st1 e1 
+         C2 st2 e2 
+         (REACH1 : <e| C1 st1 e1 ~> C2 st2 e2 |e>)=> 
+         forall C3 st3 m3 
+                (REACH2 : <e| C2 st2 e2 ~> C3 st3 m3 |m>),
+                <e| C1 st1 e1 ~> C3 st3 m3 |m>)
+    (fun C1 st1 e1 
+         C2 st2 m2 
+         (REACH1 : <e| C1 st1 e1 ~> C2 st2 m2 |m>)=> 
+         forall C3 st3 m3 
+                (REACH2 : <m| C2 st2 m2 ~> C3 st3 m3 |m>),
+                <e| C1 st1 e1 ~> C3 st3 m3 |m>)
+    (fun C1 st1 m1
+         C2 st2 e2
+         (REACH1 : <m| C1 st1 m1 ~> C2 st2 e2 |e>) =>
+         forall C3 st3 m3 
+                (REACH2 : <e| C2 st2 e2 ~> C3 st3 m3 |m>),
+                <m| C1 st1 m1 ~> C3 st3 m3 |m>)
+    (fun C1 st1 m1 
+         C2 st2 m2 
+         (REACH1 : <m| C1 st1 m1 ~> C2 st2 m2 |m>)=> 
+         forall C3 st3 m3 
+                (REACH2 : <m| C2 st2 m2 ~> C3 st3 m3 |m>),
+                <m| C1 st1 m1 ~> C3 st3 m3 |m>));
+   eauto using EreachE, EreachM, MreachE, MreachM;
+   intros; try inversion pf; subst; inversion REACH2; subst;
+   eauto using EreachE, EreachM, MreachE, MreachM.
+Qed.
+
+Lemma c_plugin_assoc : forall C1 C2 C3, C1[| C2[| C3 |] |] = ((C1[|C2|])[|C3|]).
+Proof.
+  induction C1; eauto; 
+  intros; simpl; try rewrite IHC1; eauto.
+  rewrite IHC1_2. eauto.
+Qed.
+
+Lemma eq_p_eq : forall p1 p2, eq_p p1 p2 = true <-> p1 = p2.
+Proof.
+  induction p1; induction p2;
+  intros; simpl;
+  try rewrite IHp1; try rewrite IHp2;
+  eauto.
+  - split; eauto.
+  - split; intros contra; inversion contra.
+  - split; intros contra; inversion contra.
+  - unfold eq_t. remember (a =? a0) as eqa.
+    destruct eqa; simpl; symmetry in Heqeqa;
+    try rewrite Nat.eqb_eq in Heqeqa;
+    try rewrite Nat.eqb_neq in Heqeqa.
+    + split; intros. rewrite Heqeqa in *.
+      apply IHp1 in H. rewrite H. eauto.
+      eapply IHp1. inversion H; eauto.
+    + split; intros contra; inversion contra.
+      apply Heqeqa in H0; inversion H0.
+Qed.
+
+Lemma c_plugin_adds_level : forall C1 C2, eq_p (dy_level(C1[|C2|])) (dy_level C1 ++ dy_level C2) = true.
+Proof.
+  induction C1; induction C2;
+  intros; simpl; 
+  try rewrite IHC1; try rewrite IHC2; try unfold eq_t;
+  eauto; try (assert (RR : tx =? tx = true);
+  try apply Nat.eqb_eq; eauto; try rewrite RR; try clear RR; eauto).
+  - assert (RR : dy_level (dy_c_letm M C2_1 C2_2) = dy_level C2_2); eauto;
+    rewrite <- RR; clear RR; eapply IHC1.
+  - assert (RR : dy_level (dy_c_letm M C2_1 C2_2) = dy_level C2_2); eauto;
+    rewrite <- RR; clear RR; eapply IHC1.
+  - assert (RR : dy_level (dy_c_letm M0 C2_1 C2_2) = dy_level C2_2); eauto;
+    rewrite <- RR; clear RR; eapply IHC1_2.
+Qed.
+
+(* equivalence between reachability relations *)
+Lemma Eeval_then_reach :
+    forall Ci sti ei v stv
+           (EVAL : EevalR Ci sti ei v stv)
+           ev pf Cv mem t
+           (VAL : v = Val ev pf Cv)
+           (STATE : stv = ST mem t),
+          <e| Ci sti ei ~> Cv stv ev |e>.
+Proof.
+  apply (EevalR_ind_mut
+    (fun Ci sti ei v stv
+        (EVAL : EevalR Ci sti ei v stv) =>
+        forall ev pf Cv mem t
+              (VAL : v = Val ev pf Cv)
+              (STATE : stv = ST mem t),
+        <e| Ci sti ei ~> Cv stv ev |e>)
+    (fun Ci sti mi Cv stv
+        (EVAL : MevalR Ci sti mi Cv stv) =>
+        <m| Ci sti mi ~> Cv stv m_empty |m>));
+  intros; try inversion STATE0; try inversion STATE;
+          try inversion VAL; try destruct st_lam;
+          try destruct st_m; try destruct v_e;
+          try destruct v_m1; try destruct arg; subst; 
+          eauto using EreachE, EreachM, MreachE, MreachM.
+Qed.
+
+Lemma Meval_then_reach :
+    forall Ci sti mi Cv stv
+           (EVAL : MevalR Ci sti mi Cv stv),
+           <m| Ci sti mi ~> Cv stv m_empty |m>.
+Proof.
+  apply (MevalR_ind_mut
+    (fun Ci sti ei v stv
+        (EVAL : EevalR Ci sti ei v stv) =>
+        forall ev pf Cv mem t
+              (VAL : v = Val ev pf Cv)
+              (STATE : stv = ST mem t),
+        <e| Ci sti ei ~> Cv stv ev |e>)
+    (fun Ci sti mi Cv stv
+        (EVAL : MevalR Ci sti mi Cv stv) =>
+        <m| Ci sti mi ~> Cv stv m_empty |m>));
+  intros; try inversion STATE0; try inversion STATE;
+          try inversion VAL; try destruct st_lam;
+          try destruct st_m; try destruct v_e;
+          try destruct v_m1; try destruct arg; subst; 
+          eauto using EreachE, EreachM, MreachE, MreachM.
+Qed.
+
+Lemma EreachE_equiv_left :
+    forall C1 st1 e1 C2 st2 e2,
+          <e| C1 st1 e1 ~> C2 st2 e2 |e> ->
+          _EreachE C1 st1 e1 C2 st2 e2.
+Proof.
+  apply (_EreachE_ind_mut 
+    (fun C1 st1 e1 C2 st2 e2
+        (REACH : <e| C1 st1 e1 ~> C2 st2 e2 |e>) =>
+        _EreachE C1 st1 e1 C2 st2 e2)
+    (fun C1 st1 e1 C2 st2 m2
+        (REACH : <e| C1 st1 e1 ~> C2 st2 m2 |m>) =>
+        _EreachM C1 st1 e1 C2 st2 m2)
+    (fun C1 st1 m1 C2 st2 e2
+        (REACH : <m| C1 st1 m1 ~> C2 st2 e2 |e>) =>
+        _MreachE C1 st1 m1 C2 st2 e2)
+    (fun C1 st1 m1 C2 st2 m2
+        (REACH : <m| C1 st1 m1 ~> C2 st2 m2 |m>) =>
+        _MreachM C1 st1 m1 C2 st2 m2));
+  intros; eauto using EreachE, EreachM, MreachE, MreachM, _EreachE, _MreachE, _EreachM, _MreachM.
+Qed.
+
+Lemma EreachE_equiv_right :
+    forall C1 st1 e1 C2 st2 e2,
+          _EreachE C1 st1 e1 C2 st2 e2 ->
+          <e| C1 st1 e1 ~> C2 st2 e2 |e>.
+Proof.
+  apply (__EreachE_ind_mut 
+    (fun C1 st1 e1 C2 st2 e2
+        (REACH : _EreachE C1 st1 e1 C2 st2 e2) =>
+        <e| C1 st1 e1 ~> C2 st2 e2 |e>)
+    (fun C1 st1 m1 C2 st2 e2
+        (REACH : _MreachE C1 st1 m1 C2 st2 e2) =>
+        <m| C1 st1 m1 ~> C2 st2 e2 |e>));
+  intros; try destruct v; try destruct st; try destruct st1; try destruct st_lam;
+  try destruct arg; try destruct st_m; try destruct st';
+  eauto using EreachE, EreachM, MreachE, MreachM, _EreachE, _MreachE, _EreachM, _MreachM.
+  - eapply Eeval_then_reach in FN as FNr; eauto using EreachE.
+  - eapply Eeval_then_reach in FN as FNr; eauto using EreachE.
+    eapply Eeval_then_reach in ARG as ARGr; eauto using EreachE.
+  - eapply Meval_then_reach in MOD as MODr; eauto using EreachE.
+  - eapply Eeval_then_reach in EVALx as EVALxr; eauto using MreachE.
+  - eapply Meval_then_reach in EVALM as EVALMr; eauto using MreachE.
+Qed.
+
+Theorem EreachE_equiv : 
+  forall C1 st1 e1 C2 st2 e2,
+         _EreachE C1 st1 e1 C2 st2 e2 <->
+          <e| C1 st1 e1 ~> C2 st2 e2 |e>.
+Proof. 
+  intros; split; try apply EreachE_equiv_left; try apply EreachE_equiv_right. 
+Qed.
+
+Inductive st_ctx :=
+  | st_c_hole
+  | st_c_lam (x : expr_id) (C : st_ctx)
+  | st_c_lete (x : expr_id) (C : st_ctx)
+  | st_c_letm (M : mod_id) (CM : st_ctx) (C : st_ctx)
+.
+
+Fixpoint st_level (C : st_ctx) : nat :=
+  match C with
+  | st_c_hole => 0
+  | st_c_lam _ C'
+  | st_c_lete _ C' => S (st_level C')
+  | st_c_letm _ _ C' => st_level C'
+  end.
+
+Fixpoint st_ctx_M (C : st_ctx) (M : mod_id) :=
+  match C with
+  | st_c_hole => None
+  | st_c_lam _ C'
+  | st_c_lete _ C' => st_ctx_M C' M
+  | st_c_letm M' CM' C' =>
+    match st_ctx_M C' M with
+    | Some CM => Some CM
+    | None => if eq_mid M M' then Some CM' else None
+    end
+  end.
+
+Fixpoint st_c_plugin (Cout : st_ctx) (Cin : st_ctx) :=
+  match Cout with
+  | st_c_hole => Cin
+  | st_c_lam x C' => st_c_lam x (st_c_plugin C' Cin)
+  | st_c_lete x C' => st_c_lete x (st_c_plugin C' Cin)
+  | st_c_letm M' CM' C' => st_c_letm M' CM' (st_c_plugin C' Cin)
+  end.
+
+Lemma st_c_plugin_assoc : forall C1 C2 C3,
+  st_c_plugin (st_c_plugin C1 C2) C3 =
+  st_c_plugin C1 (st_c_plugin C2 C3). 
+Proof.
+  induction C1; eauto; 
+  intros; simpl; try rewrite IHC1; eauto.
+  rewrite IHC1_2. eauto.
+Qed.
+
+Lemma st_c_plugin_add_level :
+  forall C1 C2, st_level (st_c_plugin C1 C2) = st_level C1 + st_level C2.
+Proof.
+  induction C1; induction C2; intros; simpl; eauto.
+  - assert (RR : st_level (st_c_letm M C2_1 C2_2) = st_level C2_2); eauto.
+    specialize (IHC1 (st_c_letm M C2_1 C2_2)).
+    rewrite IHC1. rewrite RR. eauto.
+  - assert (RR : st_level (st_c_letm M C2_1 C2_2) = st_level C2_2); eauto.
+    specialize (IHC1 (st_c_letm M C2_1 C2_2)).
+    rewrite IHC1. rewrite RR. eauto.
+  - assert (RR : st_level (st_c_letm M0 C2_1 C2_2) = st_level C2_2); eauto.
+    specialize (IHC1_2 (st_c_letm M0 C2_1 C2_2)).
+    rewrite IHC1_2. rewrite RR. eauto.
+Qed.
+
+Fixpoint dy_to_st C :=
+  match C with
+  |  ([||]) => st_c_hole
+  | dy_c_lam x _ C' => st_c_lam x (dy_to_st C')
+  | dy_c_lete x _ C' => st_c_lete x (dy_to_st C')
+  | dy_c_letm M CM C' => st_c_letm M (dy_to_st CM) (dy_to_st C')
+  end.
+
+Lemma dy_to_st_plugin :
+  forall Cout Cin,
+    dy_to_st (Cout[|Cin|]) = st_c_plugin (dy_to_st Cout) (dy_to_st Cin).
+Proof.
+  induction Cout; intros; simpl; try rewrite IHCout; eauto.
+  rewrite IHCout2. eauto.
+Qed. 
+
+Lemma st_ctx_M_plugin :
+  forall Cout Cin M,
+    st_ctx_M (st_c_plugin Cout Cin) M =
+      match st_ctx_M Cin M with
+      | Some CM => Some CM
+      | None =>
+        match st_ctx_M Cout M with
+        | Some CM => Some CM
+        | None => None
+        end
+      end.
+Proof.
+  induction Cout; intros; simpl; eauto.
+  - destruct (st_ctx_M Cin M); eauto.
+  - specialize (IHCout2 Cin M0). 
+    destruct (st_ctx_M Cin M0). 
+    rewrite IHCout2. eauto. 
+    rewrite IHCout2.
+    destruct (st_ctx_M Cout2 M0). eauto.
+    assert (RR : forall Cout0 Cin0, 
+    st_ctx_M (st_c_plugin Cout0 Cin0) M0 = None -> st_ctx_M Cin0 M0 = None).
+    { induction Cout0; intros; simpl; eauto. 
+      simpl in H. apply IHCout0_2.
+      destruct (st_ctx_M (st_c_plugin Cout0_2 Cin0) M0).
+      inversion H. eauto. }
+    specialize (IHCout1 Cin M0).
+    rewrite (RR Cout2 Cin IHCout2) in IHCout1.
+    destruct (eq_mid M0 M).
+    eauto. eauto.
+Qed. 
+
+Lemma mod_is_static_none : forall (dC : dy_ctx) (M : mod_id),
+  (ctx_M dC M = None <-> st_ctx_M (dy_to_st dC) M = None).
+Proof. 
+  intros. repeat split. 
+  - induction dC; simpl; eauto.
+    destruct (ctx_M dC2 M). intros H; inversion H.
+    specialize (IHdC2 eq_refl). rewrite IHdC2.
+    destruct (eq_mid M M0). intros H; inversion H. eauto.
+  - induction dC; simpl; eauto.
+    destruct (st_ctx_M (dy_to_st dC2) M). intros H; inversion H.
+    specialize (IHdC2 eq_refl). rewrite IHdC2.
+    destruct (eq_mid M M0). intros H; inversion H. eauto.
+Qed.
+
+Lemma mod_is_static_some : forall (dC : dy_ctx) (M : mod_id),
+  (forall v, ctx_M dC M = Some v -> st_ctx_M (dy_to_st dC) M = Some (dy_to_st v)) /\
+  (forall v, st_ctx_M (dy_to_st dC) M = Some v -> exists dv, dy_to_st dv = v /\ ctx_M dC M = Some dv).
+Proof.
+  intros; split. 
+  - induction dC; simpl; intros; eauto.
+    + inversion H.
+    + remember (ctx_M dC2 M) as v2. destruct v2.
+      specialize (IHdC2 v H). rewrite IHdC2. eauto.
+      symmetry in Heqv2. rewrite mod_is_static_none in Heqv2.
+      rewrite Heqv2. destruct (eq_mid M M0); inversion H; eauto.
+  - induction dC; simpl; intros; eauto.
+    + inversion H.
+    + remember (st_ctx_M (dy_to_st dC2) M) as v2. destruct v2.
+      specialize (IHdC2 v H). inversion IHdC2. exists x.
+      destruct H0. split. assumption. rewrite H1. eauto.
+      remember (ctx_M dC2 M) as v2. destruct v2;
+      symmetry in Heqv2; rewrite <- mod_is_static_none in Heqv2.
+      rewrite Heqv2 in Heqv0. inversion Heqv0.
+      destruct (eq_mid M M0). inversion H.
+      exists dC1. eauto. inversion H.
+Qed.
+
+(* Induction principle: preserves a predicate on C, st, e *)
+Lemma EreachE_ind_mut : 
+  forall (Pe : forall (C : dy_ctx) (st : state) (e : expr_tm), Prop)
+         (Pm : forall (C : dy_ctx) (st : state) (m : mod_tm), Prop),
+    (forall C st e, (Pe C st e) -> 
+      (match st with
+      | ST mem _ =>
+          forall addr,
+          match mem addr with
+            | None => True
+            | Some vl => 
+              forall v pf C_v (IN : In (Val v pf C_v) vl),
+                Pe C_v st v
+          end
+      end)) ->
+    (forall C st e1 e2,
+            Pe C st (e_app e1 e2) -> Pe C st e1) ->
+    (forall C st e1 e2 C_lam st_lam lam,
+            Pe C st (e_app e1 e2) -> 
+            Pe C_lam st_lam lam -> Pe C st_lam e2) ->
+    (forall C st e1 e2 C_lam st_lam x e
+            C_arg mem t arg pf,
+            Pe C st (e_app e1 e2) ->
+            Pe C_lam st_lam (e_lam x e) ->
+            Pe C_arg (ST mem t) arg ->
+            Pe (C_lam[|dy_c_lam x t ([||])|])
+              (ST ((dy_level C_lam ++ [t]) !-> (Val arg pf C_arg) ; mem) (update_t t)) e) ->
+    (forall C st m e, Pe C st (e_link m e) -> Pm C st m) ->
+    (forall C st m e C_m st_m,
+            Pe C st (e_link m e) -> (MevalR C st m C_m st_m) ->
+            Pm C_m st_m m_empty -> Pe C_m st_m e) ->
+    (forall C st M C_M (ACCESS : Some C_M = ctx_M C M),
+            Pm C st (m_var M) -> Pm C_M st m_empty) ->
+    (forall C st x e m,
+            Pm C st (m_lete x e m) -> Pe C st e) ->
+    (forall C st x e m C_x mem t v pf,
+            Pm C st (m_lete x e m) ->
+            Pe C_x (ST mem t) v ->
+            Pm (C[|dy_c_lete x t  ([||])|])
+              (ST ((dy_level C ++ [t]) !-> (Val v pf C_x) ; mem) (update_t t)) m) ->
+    (forall C st M m1 m2,
+            Pm C st (m_letm M m1 m2) -> Pm C st m1) ->
+    (forall C st M m1 m2 C_M st_M,
+            Pm C st (m_letm M m1 m2) ->
+            (MevalR C st m1 C_M st_M) ->
+            Pm C_M st_M m_empty ->
+            Pm (C[|dy_c_letm M C_M  ([||])|]) st_M m2) ->
+    (forall C st e C' st' e'
+            (INIT : Pe C st e)
+            (REACH : <e| C st e ~> C' st' e' |e>),
+            Pe C' st' e').
+Proof. 
+(* intros just before our goal, then fix 8, on REACH, 
+   with mutual induction on EreachM, MreachE, MreachM *)
+  intros Pe Pm MEM APPl APPr APPb LINKm LINKe MVAR LETex LETem LETm1 LETm2.
+  fix IHere 8 with 
+    (IHerm C st e C' st' m'
+          (INIT : Pe C st e)
+          (REACH : <e| C st e ~> C' st' m' |m>)
+          { struct REACH }
+          : Pm C' st' m')
+    (IHmre C st m C' st' e'
+          (INIT : Pm C st m)
+          (REACH : <m| C st m ~> C' st' e' |e>)
+          { struct REACH }
+          : Pe C' st' e')
+    (IHmrm C st m C' st' m'
+          (INIT : Pm C st m)
+          (REACH : <m| C st m ~> C' st' m' |m>)
+          { struct REACH }
+          : Pm C' st' m').
+  - intros. destruct REACH.
+    + exact INIT.
+    + specialize (MEM C st (e_var x) INIT).
+      destruct st. specialize (MEM (addr_x C x)).
+      inversion STATE; subst. rewrite <- ACCESS in MEM.
+      eapply MEM. eauto.
+    + apply (IHere C st e1 C' st' e'). eapply APPl.
+      exact INIT. exact REACH.
+    + apply (IHere C st_lam e2 C' st' e').
+      apply APPr with (st := st) (e1 := e1) (C_lam := C_lam) (lam := v).
+      exact INIT. apply (IHere C st e1 C_lam st_lam v).
+      eapply APPl. exact INIT. exact REACH1. exact REACH2.
+    + assert (LAM : Pe C_lam st_lam (e_lam x e)).
+      apply (IHere C st e1 C_lam st_lam (e_lam x e)).
+      eapply APPl. exact INIT. exact REACH1.
+      apply (IHere (C_lam [|dy_c_lam x t ([||])|])
+            (ST (dy_level C_lam ++ [t] !-> Val arg pf C_arg; mem)
+            (update_t t)) e C' st' e').
+      apply APPb with (C := C) (st := st) (e1 := e1) (e2 := e2) (st_lam := st_lam).
+      exact INIT. exact LAM. 
+      apply (IHere C st_lam e2 C_arg (ST mem t) arg).
+      apply (APPr C st e1 e2 C_lam st_lam (e_lam x e)).
+      exact INIT. exact LAM. exact REACH2. exact REACH3.
+    + apply (IHmre C st m C' st' e'). apply LINKm with (e := e). exact INIT. exact REACHm.
+    + apply (IHere C_m st_m e C' st' e'). apply LINKe with (C := C) (st := st) (m := m).
+      exact INIT. exact MOD.
+      apply (IHmrm C st m C_m st_m m_empty).
+      eapply LINKm. exact INIT. exact MODr. exact REACH.
+  - intros. destruct REACH.
+    + apply (IHerm C st e1 C' st' m'). eapply APPl.
+      exact INIT. exact REACH.
+    + apply (IHerm C st_lam e2 C' st' m').
+      eapply APPr with (C_lam := C_lam) (lam := v). exact INIT.
+      apply (IHere C st e1 C_lam st_lam v).
+      eapply APPl. exact INIT. exact FNr. exact REACH.
+    + assert (LAM : Pe C_lam st_lam (e_lam x e)).
+      apply (IHere C st e1 C_lam st_lam (e_lam x e)).
+      eapply APPl. exact INIT. exact FNr.
+      apply (IHerm (C_lam [|dy_c_lam x t ([||])|])
+            (ST (dy_level C_lam ++ [t] !-> Val arg pf C_arg; mem)
+            (update_t t)) e C' st' m').
+      eapply APPb with (st_lam := st_lam). exact INIT. exact LAM.
+      apply (IHere C st_lam e2 C_arg (ST mem t) arg).
+      apply (APPr C st e1 e2 C_lam st_lam (e_lam x e)).
+      exact INIT. exact LAM. exact ARGr. exact REACH.
+    + apply (IHmrm C st m C' st' m').
+      eapply LINKm. exact INIT. exact REACHm.
+    + apply (IHerm C_m st_m e C' st' m').
+      eapply LINKe. exact INIT. exact MOD.
+      apply (IHmrm C st m C_m st_m m_empty).
+      eapply LINKm. exact INIT. exact MODr. exact REACH.
+  - intros. destruct REACH.
+    + apply (IHere C st e C' st' e').
+      eapply LETex. exact INIT. exact REACHe.
+    + apply (IHmre (C [|dy_c_lete x t ([||])|])
+        (ST (dy_level C ++ [t] !-> Val v pf C_x; mem) (update_t t)) m
+        C' st' e').
+      eapply LETem. exact INIT.
+      apply (IHere C st e C_x (ST mem t) v).
+      eapply LETex. exact INIT. exact EVALxr. exact REACH.
+    + apply (IHmre C st m1 C' st' e').
+      eapply LETm1. exact INIT. exact REACH.
+    + apply (IHmre (C [|dy_c_letm M C_M ([||])|]) st_M m2 C' st' e').
+      eapply LETm2. exact INIT. exact EVALM.
+      apply (IHmrm C st m1 C_M st_M m_empty).
+      eapply LETm1. exact INIT. exact EVALM0. exact REACH.
+  - intros. destruct REACH.
+    + exact INIT.
+    + specialize (MVAR C st M C_M ACCESS).
+      apply MVAR. exact INIT.
+    + apply (IHerm C st e C' st' m').
+      eapply LETex. exact INIT. exact REACHe.
+    + apply (IHmrm (C [|dy_c_lete x t ([||])|])
+        (ST (dy_level C ++ [t] !-> Val v pf C_x; mem) (update_t t)) m
+        C' st' m').
+      eapply LETem. exact INIT.
+      apply (IHere C st e C_x (ST mem t) v).
+      eapply LETex. exact INIT. exact EVALxr. exact REACH.
+    + apply (IHmrm C st m1 C' st' m').
+      eapply LETm1. exact INIT. exact REACH.
+    + apply (IHmrm (C [|dy_c_letm M C_M ([||])|]) st_M m2 C' st' m').
+      eapply LETm2. exact INIT. exact EVALM.
+      apply (IHmrm C st m1 C_M st_M m_empty).
+      eapply LETm1. exact INIT. exact REACH1. exact REACH2.
+Qed.
+
+Lemma value_reach_only_itself_e :
+  forall C st v (pf : value v)
+         C' st' e'
+         (REACH : <e| C st v ~> C' st' e' |e>),
+         C = C' /\ st = st' /\ v = e'.
+Proof.
+  intros; repeat split; inversion pf; inversion REACH; subst; eauto using EreachE;
+  try inversion H0.
+Qed.
+
+Lemma value_reach_only_itself_m :
+  forall C st v (pf : value v)
+         C' st' m'
+         (REACH : <e| C st v ~> C' st' m' |m>),
+         False.
+Proof.
+  intros; repeat split; inversion pf; inversion REACH; subst; eauto using EreachM;
+  try inversion H0.
+Qed.
+
+Notation "Cout '[[|' Cin '|]]'" := (st_c_plugin Cout Cin)
+                              (at level 100, Cin at next level, right associativity).
+
+Notation "'[[||]]'" := (st_c_hole) (at level 100).
+
+(* collect all static contexts reachable from the current configuration *)
+Fixpoint collect_ctx_expr C e :=
+  match e with
+  | e_var x => [C]
+  | e_lam x e' => C :: collect_ctx_expr
+                       (C [[|st_c_lam x ([[||]]) |]]) e'
+  | e_app e1 e2 =>
+    let ctxs1 := collect_ctx_expr C e1 in
+    let ctxs2 := collect_ctx_expr C e2 in
+    ctxs1 ++ ctxs2
+  | e_link m e' =>
+    match collect_ctx_mod C m with
+    | (Some C_m, ctxs_m) => 
+      let ctxs_e := collect_ctx_expr C_m e' in
+      ctxs_m ++ ctxs_e
+    | (None, ctxs_m) => ctxs_m
+    end
+  end
+
+with collect_ctx_mod C m :=
+  match m with
+  | m_empty => (Some C, [C])
+  | m_var M =>
+    match st_ctx_M C M with
+    | Some C_M => (Some C_M, [C ; C_M])
+    | None => (None, [C])
+    end
+  | m_lete x e m' =>
+    let ctxs_e := collect_ctx_expr C e in
+    let (ctx_o, ctxs_m) := collect_ctx_mod 
+                           (C [[| st_c_lete x ([[||]]) |]]) m' in
+    (ctx_o, ctxs_e ++ ctxs_m)
+  | m_letm M m1 m2 =>
+    match collect_ctx_mod C m1 with
+    | (Some C_M, ctxs_m1) => 
+      let (ctx_o, ctxs_m2) := collect_ctx_mod
+                              (C [[| st_c_letm M C_M ([[||]]) |]]) m2 in
+      (ctx_o, ctxs_m1 ++ ctxs_m2)
+    | (None, ctxs_m1) => (None, ctxs_m1)
+    end
+  end.
+
+Compute collect_ctx_expr ([[||]]) (e_app (e_lam (eid 0) (e_var (eid 0)))
+                                  (e_lam (eid 0) (e_var (eid 0)))).
+
+Search In _ (_ ++ _).
+Search In _ (_ :: _).
+Print In.
+
+Lemma collect_ctx_expr_refl : forall e C, In C (collect_ctx_expr C e).
+Proof.
+  apply (expr_ind_mut
+    (fun e =>
+      forall C, In C (collect_ctx_expr C e))
+    (fun m =>
+      forall C, 
+        let (o, ctxs) := collect_ctx_mod C m in In C ctxs));
+  intros; simpl; eauto.
+  - apply in_app_iff. left. apply H.
+  - remember (collect_ctx_mod C m) as ol. destruct ol as [o l].
+    specialize (H C). rewrite <- Heqol in H.
+    destruct o; eauto. apply in_app_iff. left. eauto.
+  - destruct (st_ctx_M C M); simpl; left; eauto.
+  - destruct (collect_ctx_mod (C [[|st_c_lete x ([[||]])|]]) m).
+    apply in_app_iff. left. apply H.
+  - remember (collect_ctx_mod C m1) as ol.
+    destruct ol as [o l]. specialize (H C). rewrite <- Heqol in H.
+    destruct o; eauto.
+    + destruct (collect_ctx_mod (C [[|st_c_letm M s ([[||]])|]]) m2).
+      apply in_app_iff. left. eauto.
+Qed.
+
+Lemma Meval_then_collect :
+  forall C st m C_m st_m
+         (EVAL : MevalR C st m C_m st_m),
+        match collect_ctx_mod (dy_to_st C) m with
+        | (Some C_m', _) => C_m' = dy_to_st C_m
+        | (None, _) => False
+        end.
+Proof.
+  intros. induction EVAL; simpl; eauto.
+  - pose proof mod_is_static_some as H.
+    specialize (H C M). destruct H as [A B].
+    specialize (A C_M). symmetry in ACCESS.
+    specialize (A ACCESS). rewrite A. eauto.
+  - rewrite dy_to_st_plugin in IHEVAL.
+    simpl in IHEVAL.
+    remember (collect_ctx_mod (dy_to_st C [[|st_c_lete x ([[||]])|]]) m) as ol.
+    destruct ol. exact IHEVAL.
+  - rewrite dy_to_st_plugin in IHEVAL2. simpl in IHEVAL2.
+    destruct (collect_ctx_mod (dy_to_st C) m1). destruct o; try apply IHEVAL1.
+    rewrite <- IHEVAL1 in IHEVAL2.
+    destruct (collect_ctx_mod (dy_to_st C [[|st_c_letm M s ([[||]])|]]) m2).
+    exact IHEVAL2.
+Qed.
+
+Definition ctx_bound_st ub st:=
+  match st with
+  | ST mem t =>
+    forall addr,
+      match mem addr with
+      | Some vl =>
+        forall v pf C_v (INvl : In (Val v pf C_v) vl)
+               sC (IN : In sC (collect_ctx_expr (dy_to_st C_v) v)),
+               In sC ub
+      | None => True
+      end
+  end.
+
+Definition ctx_bound_expr ub C st e :=
+  ctx_bound_st ub st /\
+  forall sC (IN : In sC (collect_ctx_expr (dy_to_st C) e)),
+         In sC ub.
+
+Definition ctx_bound_mod ub C st m :=
+  ctx_bound_st ub st /\
+  let (o, ctxs) := collect_ctx_mod (dy_to_st C) m in
+  forall sC (IN : In sC ctxs),
+         In sC ub.
+
+Lemma ere_ctx_bound :
+  forall ub
+         C st e
+         C' st' e'
+         (INIT : ctx_bound_expr ub C st e)
+         (REACH : <e| C st e ~> C' st' e' |e>),
+    ctx_bound_expr ub C' st' e'.
+Proof.
+  intros ub.
+  apply (EreachE_ind_mut (ctx_bound_expr ub) (ctx_bound_mod ub)).
+  - intros. unfold ctx_bound_expr in *. destruct H as [mem expr].
+    destruct st. intros. remember (mem0 addr) as v.
+    destruct v; eauto. intros.
+    split; eauto.
+    unfold ctx_bound_st in *. specialize (mem addr).
+    rewrite <- Heqv in mem. eauto.
+  - intros. unfold ctx_bound_expr in *. destruct H as [mem expr].
+    split; eauto. intros. specialize (expr sC).
+    assert (In sC (collect_ctx_expr (dy_to_st C) (e_app e1 e2))).
+    simpl. apply in_app_iff. left. eauto. eauto.
+  - intros. unfold ctx_bound_expr in *. destruct H as [memi expri].
+    destruct H0 as [memlam exprlam]. split; eauto.
+    intros. specialize (expri sC). specialize (exprlam sC).
+    assert (In sC (collect_ctx_expr (dy_to_st C) (e_app e1 e2))).
+    simpl. apply in_app_iff. right. eauto. eauto.
+  - intros. unfold ctx_bound_expr in *. destruct H as [memi expri].
+    destruct H0 as [memlam exprlam]. destruct H1 as [memarg exprarg].
+    split. 
+    + unfold ctx_bound_st in *. unfold update_m. intro addr.
+      destruct (eq_p addr (dy_level C_lam ++ [t])).
+      remember (mem (dy_level C_lam ++ [t])) as ovl. destruct ovl.
+      * intros. specialize (memarg (dy_level C_lam ++ [t])).
+        rewrite <- Heqovl in memarg.
+        simpl in INvl. destruct INvl as [eq_arg | in_l].
+        { inversion eq_arg. apply exprarg. rewrite <- H1 in IN.
+          rewrite <- H0 in IN. eauto. }
+        { eapply memarg. eauto. eauto. }
+      * intros. simpl in INvl. destruct INvl as [eq_arg | contra]; try inversion contra.
+        inversion eq_arg. apply exprarg. rewrite <- H1 in IN.
+        rewrite <- H0 in IN. eauto.
+      * apply memarg.
+    + rewrite dy_to_st_plugin. simpl. remember (dy_to_st C_lam) as st_C.
+      simpl in exprlam. eauto.
+  - intros C st m e [mem expr]. split. exact mem.
+    simpl in expr. remember (collect_ctx_mod (dy_to_st C) m) as ol.
+    destruct ol. destruct o; intros; specialize (expr sC).
+    + assert (In sC (l ++ collect_ctx_expr s e)) as HINT.
+      apply in_app_iff. left; eauto. eauto.
+    + apply expr. eauto.
+  - intros C st m e C_m st_m [mem expr] meval [memm exprm]. split. exact memm.
+    apply Meval_then_collect in meval.
+    simpl in expr. simpl in exprm. remember (collect_ctx_mod (dy_to_st C) m) as ol.
+    destruct ol; destruct o; intros; specialize (expr sC). 
+    + rewrite <- meval in *. 
+      assert (In sC (l ++ collect_ctx_expr s e)) as HINT.
+      apply in_app_iff. right. eauto. eauto.
+    + inversion meval.
+  - intros C st M C_M ACCESS [mem expr].
+    split. exact mem. simpl in expr.
+    pose proof mod_is_static_some as MOD.
+    specialize (MOD C M). destruct MOD as [MODl MODr].
+    symmetry in ACCESS. specialize (MODl C_M ACCESS).
+    rewrite MODl in expr. simpl. intros; inversion IN; try inversion H.
+    specialize (expr (dy_to_st C_M)).
+    assert (In (dy_to_st C_M) [dy_to_st C; dy_to_st C_M]) as HINT.
+    simpl; right; eauto. eauto.
+  - intros C st x e m [mem expr].
+    split. exact mem. simpl in expr.
+    destruct (collect_ctx_mod (st_c_plugin (dy_to_st C) (st_c_lete x st_c_hole)) m).
+    intros. specialize (expr sC).
+    assert (In sC (collect_ctx_expr (dy_to_st C) e ++ l)) as HINT.
+    apply in_app_iff. left. eauto. eauto.
+  - intros C st x e m C_x mem t v pf 
+    [memi expri] [memm exprm]. split.
+    + unfold ctx_bound_st in *. unfold update_m. intro addr.
+      destruct (eq_p addr (dy_level C ++ [t])).
+      remember (mem (dy_level C ++ [t])) as ovl. destruct ovl.
+      * intros. specialize (memm (dy_level C ++ [t])).
+        rewrite <- Heqovl in memm.
+        simpl in INvl. destruct INvl as [eq_e | in_l].
+        { inversion eq_e. apply exprm. rewrite <- H1 in IN.
+          rewrite <- H0 in IN. eauto. }
+        { eapply memm. eauto. eauto. }
+      * intros. simpl in INvl. destruct INvl as [eq_e | contra]; try inversion contra.
+        inversion eq_e. apply exprm. rewrite <- H1 in IN.
+        rewrite <- H0 in IN. eauto.
+      * apply memm.
+    + simpl in expri. rewrite dy_to_st_plugin. simpl.
+      destruct (collect_ctx_mod (st_c_plugin (dy_to_st C) (st_c_lete x st_c_hole)) m).
+      intros. specialize (expri sC).
+      assert (In sC (collect_ctx_expr (dy_to_st C) e ++ l)) as HINT.
+      apply in_app_iff. right. eauto. eauto.
+  - intros C st M m1 m2 [mem expr]. split. exact mem. simpl in expr.
+    destruct (collect_ctx_mod (dy_to_st C) m1). destruct o; eauto.
+    destruct (collect_ctx_mod (st_c_plugin (dy_to_st C) (st_c_letm M s st_c_hole)) m2). destruct o;
+    intros; specialize (expr sC); 
+    assert (In sC (l ++ l0)) as HINT; try apply in_app_iff; try left; eauto.
+  - intros C st M m1 m2 C_M st_M [memi expri] meval [memm exprm].
+    apply Meval_then_collect in meval. simpl in expri. simpl in exprm.
+    remember (collect_ctx_mod (dy_to_st C) m1) as ol1. 
+    destruct ol1. destruct o; unfold ctx_bound_mod in *;
+    rewrite dy_to_st_plugin in *; simpl; split; try inversion meval; 
+    try rewrite <- meval; eauto.
+    destruct (collect_ctx_mod (dy_to_st C [[|st_c_letm M s ([[||]])|]]) m2).
+    intros. assert (In sC (l ++ l0)) as HINT. apply in_app_iff. right. eauto. eauto.
+Qed.
+
+Theorem expr_ctx_bound :
+  forall e C' st' e'
+         (REACH : <e|  ([||]) (ST empty_mem 0) e ~> C' st' e' |e>),
+         In (dy_to_st C') (collect_ctx_expr ([[||]]) e).
+Proof.
+  intros.
+  pose proof (ere_ctx_bound (collect_ctx_expr st_c_hole e)  ([||]) (ST empty_mem 0) e C' st' e') as H.
+  assert (ctx_bound_expr (collect_ctx_expr ([[||]]) e)  ([||])
+          (ST empty_mem 0) e) as FINAL.
+  - unfold ctx_bound_expr; split; simpl; eauto.
+  - apply H in FINAL; try apply REACH. 
+    destruct FINAL as [MEM KILLER].
+    apply KILLER. apply collect_ctx_expr_refl.
+Qed.
